end of day 11/08/19

formal/thy_clean.py
@@ -4,22 +4,20 @@ import re
 import os
 import sys
 
+
 def line_of_char(text, c):
     return text[:c].count("\n") + 1
 
 
-named_lemma = re.compile("lemma(s?) (\w*)(:| |=)")
-
 filename = sys.argv[1]
 if filename.endswith(".thy"):
+
     with open(filename) as file:
         text = file.read()
 
-    count = 0
-    named_lemmas = set()
-    for m in named_lemma.finditer(text):
-        count += 1
-        named_lemmas.add((line_of_char(text, m.start()), m.group(2)))
+    named_lemmas = {(line_of_char(text, m.start()), m.group(2))
+                    for m in re.finditer("lemma(s?) (\w*)(:| |=)", text)}
+    names = {m[1] for m in named_lemmas}
 
     used = set()
     for root, dirs, files in os.walk("."):
@@ -27,13 +25,16 @@ if filename.endswith(".thy"):
             if f.endswith(".thy"):
                 filepath = os.path.join(root, f)
                 with open(filepath) as search_file:
-                    for line in search_file:
-                        for line_no, name in named_lemmas.difference(used):
-                            if name in line and "lemma " not in line:
-                                used.add((line_no, name))
-    print("There are", count, "named lemmas in", filename, "of which", len(named_lemmas.difference(used)), "are unused")
+                    words = set(re.findall("(?<!lemma )\w+",
+                                           search_file.read()))
+                    named_used = names.intersection(words)
+                    used = used.union(named_used)
 
-    for line_no, name in sorted(list(named_lemmas.difference(used))):
-        print(line_no, name)
+    print("There are", len(named_lemmas), "named lemmas in", filename,
+          "of which", len(names.difference(used)), "are unused:")
+
+    unused = list({m for m in named_lemmas if m[1] not in used})
+    for line_no, name in sorted(unused):
+        print(" ", line_no, name)
 else:
     print("Invalid theory file", sys.argv[1])
