formal/GExp.thy
@@ -44,54 +44,6 @@ abbreviation gOr :: "gexp \<Rightarrow> gexp \<Rightarrow> gexp" (*infix "\<or>"
 abbreviation gAnd :: "gexp \<Rightarrow> gexp \<Rightarrow> gexp" (*infix "\<and>" 60*) where
   "gAnd v va \<equiv> Nor (Nor v v) (Nor va va)"
 
-lemma inj_gAnd: "inj gAnd"
-  apply (simp add: inj_def)
-  apply clarify
-  by (metis gexp.inject(4))
-
-lemma gAnd_determinism: "(gAnd x y = gAnd x' y') = (x = x' \<and> y = y')"
-proof
-  show "gAnd x y = gAnd x' y' \<Longrightarrow> x = x' \<and> y = y'"
-    by simp
-next
-  show "x = x' \<and> y = y' \<Longrightarrow> gAnd x y = gAnd x' y' "
-    by simp
-qed
-
-lemma gval_gAnd: "gval (gAnd g1 g2) s = (gval g1 s) \<and>\<^sub>? (gval g2 s)"
-proof(induct "gval g1 s" "gval g2 s" rule: times_trilean.induct)
-case 1
-  then show ?case
-    by (metis gval.simps(5) maybe_and_valid maybe_not_invalid maybe_or_invalid)
-next
-  case "2_1"
-  then show ?case
-    by simp
-next
-  case "2_2"
-  then show ?case
-    by simp
-next
-  case 3
-  then show ?case
-    by simp
-next
-  case "4_1"
-  then show ?case
-    by simp
-next
-  case "4_2"
-  then show ?case
-    by simp
-next
-  case 5
-  then show ?case
-    by simp
-qed
-
-lemma gval_gAnd_True: "(gval (gAnd g1 g2) s = true) = ((gval g1 s = true) \<and> gval g2 s = true)"
-  using gval_gAnd maybe_and_not_true by fastforce
-
 abbreviation Lt :: "aexp \<Rightarrow> aexp \<Rightarrow> gexp" (*infix "<" 60*) where
   "Lt a b \<equiv> Gt b a"
 
@@ -115,6 +67,18 @@ lemma gval_gOr: "gval (gOr x y) r = (gval x r) \<or>\<^sub>? (gval y r)"
 lemma gval_gNot: "gval (gNot x) s = \<not>\<^sub>? (gval x s)"
   by (simp add: maybe_or_idempotent)
 
+lemma gval_gAnd: "gval (gAnd g1 g2) s = (gval g1 s) \<and>\<^sub>? (gval g2 s)"
+  by (simp add: de_morgans_1 maybe_double_negation maybe_or_idempotent)
+
+lemma gAnd_commute: "gval (gAnd a b) s = gval (gAnd b a) s"
+  using gval_gAnd times_trilean_commutative by auto
+
+lemma gOr_commute: "gval (gOr a b) s = gval (gOr b a) s"
+  by (simp add: plus_trilean_commutative)
+
+lemma gval_gAnd_True: "(gval (gAnd g1 g2) s = true) = ((gval g1 s = true) \<and> gval g2 s = true)"
+  using gval_gAnd maybe_and_not_true by fastforce
+
 lemma nor_equiv: "gval (gNot (gOr a b)) s = gval (Nor a b) s"
   by (metis maybe_double_negation gval_gNot)
 
@@ -123,8 +87,6 @@ definition satisfiable :: "gexp \<Rightarrow> bool" where
 
 lemma unsatisfiable_false: "\<not> satisfiable (Bc False)"
   by (simp add: satisfiable_def)
-
-definition "satisfiable_list l = satisfiable (fold gAnd l (Bc True))"
 
 lemma satisfiable_true: "satisfiable (Bc True)"
   by (simp add: satisfiable_def)
@@ -149,39 +111,6 @@ case (snoc a G)
     apply (simp only: foldr.simps comp_def gval_gAnd maybe_and_true)
     by auto
 qed
-
-definition gexp_equiv :: "gexp \<Rightarrow> gexp \<Rightarrow> bool" where
-  "gexp_equiv a b \<equiv> \<forall>s. gval a s = gval b s"
-
-lemma gexp_equiv_reflexive: "gexp_equiv x x"
-  by (simp add: gexp_equiv_def)
-
-lemma gexp_equiv_symmetric: "gexp_equiv x y \<Longrightarrow> gexp_equiv y x"
-  by (simp add: gexp_equiv_def)
-
-lemma gexp_equiv_transitive: "gexp_equiv x y \<and> gexp_equiv y z \<Longrightarrow> gexp_equiv x z"
-  by (simp add: gexp_equiv_def)
-
-lemma gval_subst: "gexp_equiv x y \<Longrightarrow> P (gval x s) \<Longrightarrow> P (gval y s)"
-  by (simp add: gexp_equiv_def)
-
-lemma gexp_equiv_satisfiable: "gexp_equiv x y \<Longrightarrow> satisfiable x = satisfiable y"
-  by (simp add: gexp_equiv_def satisfiable_def)
-
-lemma gAnd_reflexivity: "gexp_equiv (gAnd x x) x"
-  by (simp add: gexp_equiv_def maybe_double_negation maybe_or_idempotent)
-
-lemma gAnd_zero: "gexp_equiv (gAnd (Bc True) x) x"
-  apply (simp add: gexp_equiv_def)
-  apply (rule allI)
-  apply (case_tac "gval x s")
-  by simp_all
-
-lemma gAnd_symmetry: "gexp_equiv (gAnd x y) (gAnd y x)"
-  by (simp add: add.commute gexp_equiv_def)
-
-lemma satisfiable_gAnd_self: "satisfiable (gAnd x x) = satisfiable x"
-  by (simp add: gAnd_reflexivity gexp_equiv_satisfiable)
 
 fun gexp_constrains :: "gexp \<Rightarrow> aexp \<Rightarrow> bool" where
   "gexp_constrains (gexp.Bc _) _ = False" |
@@ -216,101 +145,74 @@ next
 qed
 
 fun enumerate_gexp_inputs :: "gexp \<Rightarrow> nat set" where
-  "enumerate_gexp_inputs (GExp.Bc _) = {}" |
-  "enumerate_gexp_inputs (GExp.Null v) = enumerate_aexp_inputs v" |
-  "enumerate_gexp_inputs (GExp.Eq v va) = enumerate_aexp_inputs v \<union> enumerate_aexp_inputs va" |
-  "enumerate_gexp_inputs (GExp.Lt v va) = enumerate_aexp_inputs v \<union> enumerate_aexp_inputs va" |
-  "enumerate_gexp_inputs (GExp.Nor v va) = enumerate_gexp_inputs v \<union> enumerate_gexp_inputs va"
+  "enumerate_gexp_inputs (Bc _) = {}" |
+  "enumerate_gexp_inputs (Null v) = enumerate_aexp_inputs v" |
+  "enumerate_gexp_inputs (Eq v va) = enumerate_aexp_inputs v \<union> enumerate_aexp_inputs va" |
+  "enumerate_gexp_inputs (Lt v va) = enumerate_aexp_inputs v \<union> enumerate_aexp_inputs va" |
+  "enumerate_gexp_inputs (Nor v va) = enumerate_gexp_inputs v \<union> enumerate_gexp_inputs va"
 
-fun enumerate_gexp_inputs_list :: "gexp \<Rightarrow> nat list" where
-  "enumerate_gexp_inputs_list (GExp.Bc _) = []" |
-  "enumerate_gexp_inputs_list (GExp.Null v) = enumerate_aexp_inputs_list v" |
-  "enumerate_gexp_inputs_list (GExp.Eq v va) = enumerate_aexp_inputs_list v @ enumerate_aexp_inputs_list va" |
-  "enumerate_gexp_inputs_list (GExp.Lt v va) = enumerate_aexp_inputs_list v @ enumerate_aexp_inputs_list va" |
-  "enumerate_gexp_inputs_list (GExp.Nor v va) = enumerate_gexp_inputs_list v @ enumerate_gexp_inputs_list va"
-
-lemma enumerate_gexp_inputs_list: "enumerate_gexp_inputs l = set (enumerate_gexp_inputs_list l)"
-proof(induct l)
+lemma enumerate_gexp_inputs_list: "\<exists>l. enumerate_gexp_inputs g = set l"
+proof(induct g)
 case (Bc x)
   then show ?case
     by simp
 next
   case (Eq x1a x2)
   then show ?case
-    by (simp add: enumerate_aexp_inputs_list)
+    by (metis enumerate_aexp_inputs_list enumerate_gexp_inputs.simps(3) set_union)
 next
   case (Gt x1a x2)
   then show ?case
-    by (simp add: enumerate_aexp_inputs_list)
+    by (metis enumerate_aexp_inputs_list enumerate_gexp_inputs.simps(4) set_union)
 next
   case (Nor l1 l2)
   then show ?case
-    by simp
+    by (metis enumerate_gexp_inputs.simps(5) set_union_append)
 next
   case (Null x)
   then show ?case
     by (simp add: enumerate_aexp_inputs_list)
 qed
 
-lemma set_enumerate_gexp_inputs_list:
-"set (fold (@) (map enumerate_gexp_inputs_list l) []) = (\<Union> (set (map enumerate_gexp_inputs l)))"
-proof(induct l)
-case Nil
-  then show ?case
-    by simp
-next
-case (Cons a l)
-  then show ?case
-    using enumerate_gexp_inputs_list
-    by (simp add: fold_append_concat_rev inf_sup_aci(5))
-qed
-
 definition max_input :: "gexp \<Rightarrow> nat option" where
   "max_input g = (let inputs = (enumerate_gexp_inputs g) in if inputs = {} then None else Some (Max inputs))"
 
 definition max_input_list :: "gexp list \<Rightarrow> nat option" where
-  "max_input_list g = (fold max (map (\<lambda>g. GExp.max_input g) g) None)"
+  "max_input_list g = (fold max (map (\<lambda>g. max_input g) g) None)"
 
-lemma max_input_list_cons: "max_input_list (a # G) = max (GExp.max_input a) (max_input_list G)"
+lemma max_input_list_cons: "max_input_list (a # G) = max (max_input a) (max_input_list G)"
   apply (simp add: max_input_list_def)
 proof -
-  have "foldr max (GExp.max_input a # rev (map_tailrec GExp.max_input G)) None = foldr max (rev (None # map_tailrec GExp.max_input G)) (GExp.max_input a)"
+  have "foldr max (max_input a # rev (map_tailrec max_input G)) None = foldr max (rev (None # map_tailrec max_input G)) (max_input a)"
     by (metis (no_types) Max.set_eq_fold comp_def fold.simps(2) fold_conv_foldr foldr_conv_fold list.set(2) max.commute set_rev)
-  then show "fold max (map GExp.max_input G) (max (GExp.max_input a) None) = max (GExp.max_input a) (fold max (map GExp.max_input G) None)"
+  then show "fold max (map max_input G) (max (max_input a) None) = max (max_input a) (fold max (map max_input G) None)"
     by (simp add: fold_conv_foldr map_eq_map_tailrec max.commute)
 qed
 
 fun enumerate_gexp_regs :: "gexp \<Rightarrow> nat set" where
-  "enumerate_gexp_regs (GExp.Bc _) = {}" |
-  "enumerate_gexp_regs (GExp.Null v) = enumerate_aexp_regs v" |
-  "enumerate_gexp_regs (GExp.Eq v va) = enumerate_aexp_regs v \<union> enumerate_aexp_regs va" |
-  "enumerate_gexp_regs (GExp.Lt v va) = enumerate_aexp_regs v \<union> enumerate_aexp_regs va" |
-  "enumerate_gexp_regs (GExp.Nor v va) = enumerate_gexp_regs v \<union> enumerate_gexp_regs va"
+  "enumerate_gexp_regs (Bc _) = {}" |
+  "enumerate_gexp_regs (Null v) = enumerate_aexp_regs v" |
+  "enumerate_gexp_regs (Eq v va) = enumerate_aexp_regs v \<union> enumerate_aexp_regs va" |
+  "enumerate_gexp_regs (Lt v va) = enumerate_aexp_regs v \<union> enumerate_aexp_regs va" |
+  "enumerate_gexp_regs (Nor v va) = enumerate_gexp_regs v \<union> enumerate_gexp_regs va"
 
-fun enumerate_gexp_regs_list :: "gexp \<Rightarrow> nat list" where
-  "enumerate_gexp_regs_list (GExp.Bc _) = []" |
-  "enumerate_gexp_regs_list (GExp.Null v) = enumerate_aexp_regs_list v" |
-  "enumerate_gexp_regs_list (GExp.Eq v va) = enumerate_aexp_regs_list v @ enumerate_aexp_regs_list va" |
-  "enumerate_gexp_regs_list (GExp.Lt v va) = enumerate_aexp_regs_list v @ enumerate_aexp_regs_list va" |
-  "enumerate_gexp_regs_list (GExp.Nor v va) = enumerate_gexp_regs_list v @ enumerate_gexp_regs_list va"
-
-lemma enumerate_gexp_regs_list: "set (enumerate_gexp_regs_list l) = enumerate_gexp_regs l"
-proof(induct l)
+lemma enumerate_gexp_regs_list: "\<exists>l. enumerate_gexp_regs g = set l"
+proof(induct g)
 case (Bc x)
   then show ?case
     by simp
 next
   case (Eq x1a x2)
   then show ?case
-    by (simp add: enumerate_aexp_regs_list)
+    by (metis enumerate_aexp_regs_list enumerate_gexp_regs.simps(3) set_union_append)
 next
   case (Gt x1a x2)
   then show ?case
-    by (simp add: enumerate_aexp_regs_list)
+    by (metis enumerate_aexp_regs_list enumerate_gexp_regs.simps(4) set_append)
 next
   case (Nor l1 l2)
   then show ?case
-    by simp
+    by (metis enumerate_gexp_regs.simps(5) set_append)
 next
   case (Null x)
   then show ?case
@@ -318,8 +220,8 @@ next
 qed
 
 lemma no_variables_list_gval:
-  "enumerate_gexp_inputs_list g = [] \<Longrightarrow>
-   enumerate_gexp_regs_list g = [] \<Longrightarrow>
+  "enumerate_gexp_inputs g = {} \<Longrightarrow>
+   enumerate_gexp_regs g = {} \<Longrightarrow>
    gval g s = gval g s'"
 proof(induct g)
 case (Bc x)
@@ -328,11 +230,11 @@ case (Bc x)
 next
   case (Eq x1a x2)
   then show ?case
-    by (metis append_is_Nil_conv enumerate_gexp_inputs_list.simps(3) enumerate_gexp_regs_list.simps(3) gval.simps(4) no_variables_list_aval)
+    by (metis Un_empty enumerate_gexp_inputs.simps(3) enumerate_gexp_regs.simps(3) gval.simps(4) no_variables_aval)
 next
   case (Gt x1a x2)
   then show ?case
-    by (metis Nil_is_append_conv enumerate_gexp_inputs_list.simps(4) enumerate_gexp_regs_list.simps(4) gval.simps(3) no_variables_list_aval)
+    by (metis Un_empty enumerate_gexp_inputs.simps(4) enumerate_gexp_regs.simps(4) gval.simps(3) no_variables_aval)
 next
   case (Nor a1 a2)
   then show ?case
@@ -340,79 +242,33 @@ next
 next
   case (Null x)
   then show ?case
-    by (metis enumerate_gexp_inputs_list.simps(2) enumerate_gexp_regs_list.simps(2) gval.simps(6) no_variables_list_aval)
+    by (metis enumerate_gexp_inputs.simps(2) enumerate_gexp_regs.simps(2) gval.simps(6) no_variables_aval)
 qed
 
 lemma no_variables_list_valid_or_unsat:
-  "enumerate_gexp_inputs_list g = [] \<Longrightarrow>
-   enumerate_gexp_regs_list g = [] \<Longrightarrow>
+  "enumerate_gexp_inputs g = {} \<Longrightarrow>
+   enumerate_gexp_regs g = {} \<Longrightarrow>
    valid g \<or> \<not> satisfiable g"
 proof(induct g)
-case (Bc x)
+  case (Bc x)
   then show ?case
-    apply (cases x)
-     apply (simp add: valid_true)
-    by (simp add: unsatisfiable_false)
-next
-case (Eq x1a x2)
-  then show ?case
-    apply (simp add: valid_def satisfiable_def)
-    by (metis no_variables_list_aval)
-next
-case (Gt x1a x2)
-  then show ?case
-    apply (simp add: valid_def satisfiable_def)
-    by (metis no_variables_list_aval)
-next
-  case (Nor g1 g2)
-  then show ?case
-    apply (simp add: valid_def satisfiable_def)
-    by (metis no_variables_list_gval)
-next
-  case (Null x)
-  then show ?case
-    apply (simp add: valid_def satisfiable_def)
-    by (metis no_variables_list_aval)
-qed
-
-lemma gval_ir_take: "A \<le> length i \<Longrightarrow>
-      enumerate_gexp_regs_list a = [] \<Longrightarrow>
-      enumerate_gexp_inputs_list a \<noteq> [] \<Longrightarrow>
-      foldr max (enumerate_gexp_inputs_list a) 0 < A \<Longrightarrow>
-      gval a (join_ir (take A i) r) = gval a (join_ir i ra)"
-proof(induct a)
-case (Bc x)
-  then show ?case
-    by simp
+    by (metis (full_types) unsatisfiable_false valid_true)
 next
   case (Eq x1a x2)
   then show ?case
-    apply simp
-    apply (case_tac "enumerate_aexp_inputs_list x1a = []")
-     apply simp
-     apply (metis aval_ir_take no_variables_list_aval)
-    apply simp
-    by (metis Eq.prems(1) Eq.prems(4) List.finite_set Max.set_eq_fold Max_insert aval_ir_take fold_simps(1) foldr_conv_fold list.set(2) max.commute max_0L max_less_iff_conj no_variables_list_aval set_empty set_rev)
+    by (metis no_variables_list_gval satisfiable_def valid_def)
 next
   case (Gt x1a x2)
   then show ?case
-    apply simp
-    apply (case_tac "enumerate_aexp_inputs_list x1a = []")
-     apply simp
-     apply (metis aval_ir_take no_variables_list_aval)
-    apply simp
-    by (metis List.finite_set Max.set_eq_fold Max_insert aval_ir_take foldr.simps(1) foldr_conv_fold id_apply list.set(2) max_less_iff_conj no_variables_list_aval set_empty set_rev)
+    by (metis no_variables_list_gval satisfiable_def valid_def)
 next
-  case (Nor a1 a2)
+  case (Nor g1 g2)
   then show ?case
-    apply simp
-    apply clarify
-    by (metis List.finite_set Max.set_eq_fold Max_insert foldr.simps(1) foldr_conv_fold id_apply list.set(2) max_less_iff_conj no_variables_list_gval set_empty set_rev)
+    by (metis no_variables_list_gval satisfiable_def valid_def)
 next
   case (Null x)
   then show ?case
-    apply simp
-    by (metis aval_ir_take)
+    by (metis no_variables_list_gval satisfiable_def valid_def)
 qed
 
 definition max_reg :: "gexp \<Rightarrow> nat option" where
@@ -434,9 +290,9 @@ lemma max_reg_Nor: "max_reg (Nor a b) = max (max_reg a) (max_reg b)"
   by (metis List.finite_set Max.union enumerate_gexp_regs_list)
 
 lemma max_reg_Null: "max_reg (Null a) = AExp.max_reg a"
-  by (simp add: AExp.max_reg_def GExp.max_reg_def)
+  by (simp add: AExp.max_reg_def max_reg_def)
 
-lemma no_reg_gval_swap_regs: "GExp.max_reg g = None \<Longrightarrow> gval g (join_ir i r) = gval g (join_ir i r')"
+lemma no_reg_gval_swap_regs: "max_reg g = None \<Longrightarrow> gval g (join_ir i r) = gval g (join_ir i r')"
 proof(induct g)
 case (Bc x)
   then show ?case
@@ -482,93 +338,6 @@ next
     by (simp add: enumerate_aexp_regs_empty_reg_unconstrained)
 qed
 
-lemma enumerate_gexp_regs_set_reg_unconstrained:
-  "\<forall>x\<in>set G. enumerate_gexp_regs x = {} \<Longrightarrow>
-   \<forall>r. \<forall>g\<in>set G. \<not> gexp_constrains g (V (R r))"
-  by (simp add: enumerate_gexp_regs_empty_reg_unconstrained)
-
-lemma enumerate_gexp_inputs_empty_input_unconstrained:
-  "enumerate_gexp_inputs g = {} \<Longrightarrow>
-   \<forall>r. \<not> gexp_constrains g (V (vname.I r))"
-proof(induct g)
-case (Bc x)
-  then show ?case
-    by simp
-next
-  case (Eq x1a x2)
-  then show ?case
-    by (simp add: enumerate_aexp_inputs_empty_input_unconstrained)
-next
-  case (Gt x1a x2)
-  then show ?case
-    by (simp add: enumerate_aexp_inputs_empty_input_unconstrained)
-next
-  case (Nor g1 g2)
-  then show ?case
-    by simp
-next
-  case (Null x)
-  then show ?case
-    by (simp add: enumerate_aexp_inputs_empty_input_unconstrained)
-qed
-
-lemma enumerate_gexp_inputs_set_input_unconstrained:
-  "\<forall>x\<in>set G. enumerate_gexp_inputs x = {} \<Longrightarrow>
-   \<forall>r. \<forall>g\<in>set G. \<not> gexp_constrains g (V (vname.I r))"
-  by (simp add: enumerate_gexp_inputs_empty_input_unconstrained)
-
-lemma input_unconstrained_gval_input_swap:
-  "\<forall>r. \<not> gexp_constrains a (V (vname.I r)) \<Longrightarrow>
-  (gval a (join_ir i r) = gval a (join_ir i' r))"
-proof(induct a)
-  case (Bc x)
-  then show ?case
-    by (simp add: no_variables_list_gval)
-next
-  case (Eq x1a x2)
-  then show ?case
-    apply (simp add: ValueEq_def)
-    by (metis input_unconstrained_aval_input_swap)
-next
-  case (Gt x1a x2)
-  then show ?case
-    apply (simp add: ValueGt_def)
-    by (metis input_unconstrained_aval_input_swap)
-next
-  case (Nor a1 a2)
-  then show ?case
-    by simp
-next
-  case (Null x)
-  then show ?case
-    by (metis gexp_constrains.simps(2) gval.simps(6) input_unconstrained_aval_input_swap)
-qed
-
-lemma register_unconstrained_gval_register_swap: "\<forall>r. \<not> gexp_constrains a (V (R r)) \<Longrightarrow> (gval a (join_ir i r) = gval a (join_ir i r'))"
-proof(induct a)
-  case (Bc x)
-  then show ?case
-    by (simp add: no_variables_list_gval)
-next
-  case (Eq x1a x2)
-  then show ?case
-    apply (simp add: ValueEq_def)
-    by (metis input_unconstrained_aval_register_swap)
-next
-  case (Gt x1a x2)
-  then show ?case
-    apply (simp add: ValueGt_def)
-    by (metis input_unconstrained_aval_register_swap)
-next
-  case (Nor a1 a2)
-  then show ?case
-    by simp
-next
-  case (Null x)
-  then show ?case
-    by (metis gexp.distinct(13) gexp.distinct(17) gexp.distinct(19) gexp.distinct(7) gexp.inject(5) gexp_constrains.simps(2) gval.elims input_unconstrained_aval_register_swap)
-qed
-
 lemma unconstrained_variable_swap_gval:
    "\<forall>r. \<not> gexp_constrains g (V (vname.I r)) \<Longrightarrow>
     \<forall>r. \<not> gexp_constrains g (V (R r)) \<Longrightarrow>
@@ -595,18 +364,6 @@ next
     by (metis gexp_constrains.simps(2) gval.simps(6) unconstrained_variable_swap_aval)
 qed
 
-lemma gval_foldr_map_gval: "gval (foldr gAnd G (Bc True)) s = foldr (\<and>\<^sub>?) (map (\<lambda>g. gval g s) G) true"
-proof(induct G)
-  case Nil
-  then show ?case
-    by simp
-next
-  case (Cons a G)
-  then show ?case
-    apply (simp only: foldr.simps comp_def gval_gAnd)
-    by simp
-qed
-
 lemma gval_In_cons: "gval (In v (a # as)) s = (gval (Eq (V v) (L a)) s \<or>\<^sub>? gval (In v as) s)"
   apply (cases as)
    apply (simp add: ValueEq_def)
@@ -624,18 +381,10 @@ next
     by (metis In.simps(1) ValueEq_def add.commute gval.simps(2) join_ir_double_exists maybe_or_idempotent plus_trilean.simps(6))
 qed
 
-lemma gAnd_commute: "gval (gAnd a b) s = gval (gAnd b a) s"
-  using gval_gAnd times_trilean_commutative by auto
-
-fun null_guard :: "gexp \<Rightarrow> bool" where
-  "null_guard (Null _) = True" |
-  "null_guard (Nor g1 g2) = (null_guard g1 \<or> null_guard g2)" |
-  "null_guard _ = False"
-
 definition max_reg_list :: "gexp list \<Rightarrow> nat option" where
-  "max_reg_list g = (fold max (map (\<lambda>g. GExp.max_reg g) g) None)"
+  "max_reg_list g = (fold max (map (\<lambda>g. max_reg g) g) None)"
 
-lemma max_reg_list_cons: "max_reg_list (a # G) = max (GExp.max_reg a) (max_reg_list G)"
+lemma max_reg_list_cons: "max_reg_list (a # G) = max (max_reg a) (max_reg_list G)"
   apply (simp add: max_reg_list_def)
   by (metis (no_types, lifting) List.finite_set Max.insert Max.set_eq_fold fold.simps(1) id_apply list.simps(15) max.assoc set_empty)
 
@@ -721,22 +470,6 @@ next
     by auto
 qed
 
-lemma apply_guards_swap:
-  "apply_guards G (join_ir i r) \<Longrightarrow>
-   \<forall>x\<in>set G. enumerate_gexp_regs x = {} \<Longrightarrow>
-   \<forall>x\<in>set G. enumerate_gexp_inputs x = {} \<Longrightarrow>
-   apply_guards G (join_ir i' r')"
-proof(induct G)
-  case Nil
-  then show ?case
-    by (simp add: apply_guards_def)
-next
-  case (Cons a G)
-  then show ?case
-    apply (simp add: apply_guards_cons)
-    by (metis enumerate_gexp_inputs_list enumerate_gexp_regs_list no_variables_list_gval set_empty)
-qed
-
 lemma valid_list_apply_guards: "valid_list G \<Longrightarrow> apply_guards G s"
   by (simp add: apply_guards_def valid_list_all_valid valid_def)
 
@@ -744,78 +477,36 @@ lemma apply_guards_rearrange: "x \<in> set G \<Longrightarrow> apply_guards G s 
   apply (simp add: apply_guards_def)
   by auto
 
-lemma unconstrained_variable_swap:
-  "\<forall>r. \<forall>g\<in>set G. \<not> gexp_constrains g (V (vname.I r)) \<Longrightarrow>
-   \<forall>r. \<forall>g\<in>set G. \<not> gexp_constrains g (V (R r)) \<Longrightarrow>
-   apply_guards G s = apply_guards G s'"
-proof(induct G)
-  case Nil
-  then show ?case
-    by (simp add: apply_guards_def)
-next
-  case (Cons a G)
-  then show ?case
-    unfolding apply_guards_def
-    apply simp
-    by (metis unconstrained_variable_swap_gval)
-qed
+lemma max_input_Bc: "max_input (Bc x) = None"
+  by (simp add: max_input_def)
 
-lemma unconstrained_variable_swap_apply_guards:
-  "\<forall>r. \<forall>g\<in>set G. \<not> gexp_constrains g (V (vname.I r)) \<Longrightarrow>
-   \<forall>r. \<forall>g\<in>set G. \<not> gexp_constrains g (V (R r)) \<Longrightarrow>
-   gval (foldr gAnd G (Bc True)) s = true \<Longrightarrow>
-   apply_guards G s'"
-proof(induct G)
-  case Nil
-  then show ?case
-    by (simp add: apply_guards_def)
-next
-  case (Cons a G)
-  then show ?case
-    apply (simp only: foldr.simps comp_def gval_gAnd maybe_and_true apply_guards_cons)
-    apply simp
-    by (metis unconstrained_variable_swap_gval)
-qed
-
-lemma max_lt_val: "max (GExp.max_input a) (max_input_list G) = Some i \<Longrightarrow> (GExp.max_input a) \<le> Some i"
-  by (metis max.cobounded1)
-
-lemma max_input_Bc: "GExp.max_input (Bc x) = None"
-  by (simp add: GExp.max_input_def)
-
-lemma gexp_max_input_nor: "GExp.max_input (Nor g1 g2) = max (GExp.max_input g1) (GExp.max_input g2)"
-  apply (simp add: GExp.max_input_def Let_def)
-  apply safe
-    apply (simp add: max_None_l)
-   apply (simp add: max.commute max_None_l)
-  by (metis List.finite_set Max.union enumerate_gexp_inputs_list max_Some_Some)
-
-lemma max_input_Eq: "GExp.max_input (Eq a1 a2) = max (AExp.max_input a1) (AExp.max_input a2)"
-  apply (simp add: AExp.max_input_def GExp.max_input_def Let_def)
+lemma max_input_Eq: "max_input (Eq a1 a2) = max (AExp.max_input a1) (AExp.max_input a2)"
+  apply (simp add: AExp.max_input_def max_input_def Let_def)
   apply safe
     apply (simp add: max_None_l)
    apply (simp add: max.commute max_None_l)
   by (metis List.finite_set Max.union enumerate_aexp_inputs_list max_Some_Some)
 
-lemma max_reg_list_Eq: "GExp.max_reg (Eq a1 a2) = max (AExp.max_reg a1) (AExp.max_reg a2)"
-  apply (simp add: AExp.max_reg_def GExp.max_reg_def Let_def)
-  apply safe
-    apply (simp add: max_None_l)
-   apply (simp add: max.commute max_None_l)
-  by (metis List.finite_set Max.union enumerate_aexp_regs_list max_Some_Some)
-
-lemma max_input_Gt: "GExp.max_input (Gt a1 a2) = max (AExp.max_input a1) (AExp.max_input a2)"
-  apply (simp add: AExp.max_input_def GExp.max_input_def Let_def)
+lemma max_input_Gt: "max_input (Gt a1 a2) = max (AExp.max_input a1) (AExp.max_input a2)"
+  apply (simp add: AExp.max_input_def max_input_def Let_def)
   apply safe
     apply (simp add: max_None_l)
    apply (simp add: max.commute max_None_l)
   by (metis List.finite_set Max.union enumerate_aexp_inputs_list max.commute max_Some_Some)
 
-lemma gexp_max_input_Null: "GExp.max_input (Null x) = AExp.max_input x"
-  by (simp add: AExp.max_input_def GExp.max_input_def)
+lemma gexp_max_input_Nor: "max_input (Nor g1 g2) = max (max_input g1) (max_input g2)"
+  apply (simp add: max_input_def Let_def)
+  apply safe
+    apply (simp add: max_None_l)
+   apply (simp add: max.commute max_None_l)
+  by (metis List.finite_set Max.union enumerate_gexp_inputs_list max_Some_Some)
 
-lemma gval_take: "GExp.max_input g < Some a \<Longrightarrow>
-    gval g (join_ir i r) = gval g (join_ir (take a i) r)"
+lemma gexp_max_input_Null: "max_input (Null x) = AExp.max_input x"
+  by (simp add: AExp.max_input_def max_input_def)
+
+lemma gval_take:
+  "max_input g < Some a \<Longrightarrow>
+   gval g (join_ir i r) = gval g (join_ir (take a i) r)"
 proof(induct g)
 case (Bc x)
   then show ?case
@@ -831,20 +522,16 @@ next
 next
   case (Nor g1 g2)
   then show ?case
-    by (simp add: maybe_not_eq gexp_max_input_nor)
+    by (simp add: maybe_not_eq gexp_max_input_Nor)
 next
   case (Null x)
   then show ?case
     by (metis aval_take gexp_max_input_Null gval.simps(6))
 qed
 
-lemma gval_take_flip: "GExp.max_input g < Some a \<Longrightarrow>
-    gval g (join_ir (take a i) r) = gval g (join_ir i r)"
-  by (metis gval_take)
-
 lemma gval_no_reg_swap_regs:
-  "GExp.max_input g < Some a \<Longrightarrow>
-   GExp.max_reg g = None \<Longrightarrow>
+  "max_input g < Some a \<Longrightarrow>
+   max_reg g = None \<Longrightarrow>
    gval g (join_ir i ra) = gval g (join_ir (take a i) r)"
 proof(induct g)
 case (Bc x)
@@ -861,22 +548,11 @@ next
 next
   case (Nor g1 g2)
   then show ?case
-    by (simp add: gexp_max_input_nor max_reg_Nor max_is_None)
+    by (simp add: gexp_max_input_Nor max_reg_Nor max_is_None)
 next
   case (Null x)
   then show ?case
     by (metis gval_take no_reg_gval_swap_regs)
-qed
-
-lemma max_reg_list_none_set: "(max_reg_list G = None) = (\<forall>g \<in> set G. GExp.max_reg g = None)"
-proof(induct G)
-  case Nil
-  then show ?case
-    by (simp add: max_reg_list_def)
-next
-  case (Cons a G)
-  then show ?case
-    by (simp add: max_reg_list_cons max_is_None)
 qed
 
 lemma gval_fold_gAnd_append_singleton:
@@ -982,18 +658,6 @@ lemma gval_fold_rev_equiv_fold: "gval (fold gAnd (rev G) (Bc True)) s =  gval (f
 
 lemma gval_fold_equiv_fold_rev: "gval (fold gAnd G (Bc True)) s = gval (fold gAnd (rev G) (Bc True)) s"
   by (simp add: gval_fold_rev_equiv_fold)
-
-lemma gval_fold_gAnd: "gval (fold gAnd G (Bc True)) s = fold (\<and>\<^sub>?) (map (\<lambda>g. gval g s) G) true"
-proof(induct G rule: rev_induct)
-  case Nil
-  then show ?case
-    by simp
-next
-  case (snoc a G)
-  then show ?case
-    apply (simp add: fold_conv_foldr del: foldr.simps)
-    by (simp only: foldr.simps comp_def gval_gAnd)
-qed
 
 lemma gval_fold_equiv_gval_foldr: "gval (fold gAnd G (Bc True)) s = gval (foldr gAnd G (Bc True)) s"
 proof -
@@ -1130,17 +794,6 @@ next
   case (Cons g gs)
   then show ?case
     by (metis apply_guards_cons gval_no_reg_swap_regs max.strict_boundedE max_input_list_cons max_is_None max_reg_list_cons not_null_length take_or_pad_def)
-qed
-
-lemma max_reg_list_ensure_not_null: "max_reg_list (ensure_not_null a) = None"
-proof(induct a)
-  case 0
-  then show ?case
-    by (simp add: ensure_not_null_def max_reg_list_def)
-next
-  case (Suc a)
-  then show ?case
-    by (simp add: ensure_not_null_cons max_reg_list_append max_reg_list_def max_reg_gNot max_reg_Null max_reg_V)
 qed
 
 lemma apply_guards_ensure_not_null:
