formal/inference/Code_Target_FSet.thy
@@ -11,7 +11,7 @@ lemma fprod_code [code]:
   apply (simp add: fprod_def fset_of_list_def fset_both_sides Abs_fset_inverse)
   by auto
 
-lemma fminus_fset_filter[code]: "fset_of_list A -  xs = fset_of_list (filter (\<lambda>x. x |\<notin>| xs) A)"
+lemma fminus_fset_filter [code]: "fset_of_list A -  xs = fset_of_list (filter (\<lambda>x. x |\<notin>| xs) A)"
   by auto
 
 lemma sup_fset_foldr: "f1 |\<union>| (fset_of_list f2) = foldr finsert f2 f1"
@@ -25,19 +25,19 @@ next
     by (simp add: finsert_def sup_fset_def fset_both_sides Abs_fset_inverse)
 qed
 
-lemma sup_fset_fold: "f1 |\<union>| (fset_of_list f2) = fold finsert f2 f1"
+lemma sup_fset_fold [code]: "f1 |\<union>| (fset_of_list f2) = fold finsert f2 f1"
   by (metis foldr_conv_fold fset_of_list_rev rev_rev_ident sup_fset_foldr)
 
-lemma sup_fset_fold_double[code]: "(fset_of_list f1) |\<union>| (fset_of_list f2) = fset_of_list (f1@f2)"
+lemma sup_fset_fold_double [code]: "(fset_of_list f1) |\<union>| (fset_of_list f2) = fset_of_list (f1@f2)"
   by simp
 
-lemma bot_fset[code]: "{||} = fset_of_list []"
+lemma bot_fset [code]: "{||} = fset_of_list []"
   by simp
 
-lemma finsert_cons[code]: "finsert a (fset_of_list as) = fset_of_list (a#as)"
+lemma finsert_cons [code]: "finsert a (fset_of_list as) = fset_of_list (a#as)"
   by simp
 
-lemma ffilter_filter[code]: "ffilter f (fset_of_list as) = fset_of_list (List.filter f as)"
+lemma ffilter_filter [code]: "ffilter f (fset_of_list as) = fset_of_list (List.filter f as)"
 proof(induct as)
   case Nil
   then show ?case
@@ -48,7 +48,7 @@ next
     by auto
 qed
 
-lemma fimage_map[code]: "fimage f (fset_of_list as) = fset_of_list (List.map f as)"
+lemma fimage_map [code]: "fimage f (fset_of_list as) = fset_of_list (List.map f as)"
 proof(induct as)
   case Nil
   then show ?case
@@ -70,16 +70,16 @@ next
     by auto
 qed
 
-lemma ffUnion_fold[code]: "ffUnion (fset_of_list as) = fold (|\<union>|) as {||}"
+lemma ffUnion_fold [code]: "ffUnion (fset_of_list as) = fold (|\<union>|) as {||}"
   by (simp add: fold_union_ffUnion)
 
-lemma fmember[code]: "a |\<in>| (fset_of_list as) = List.member as a"
+lemma fmember [code]: "a |\<in>| (fset_of_list as) = List.member as a"
   by (simp add: fset_of_list_elem member_def)
 
-lemma fthe_elem[code]: "fthe_elem (fset_of_list [x]) = x"
+lemma fthe_elem [code]: "fthe_elem (fset_of_list [x]) = x"
   by simp
 
-lemma size[code]: "size (fset_of_list as) = length (remdups as)"
+lemma size [code]: "size (fset_of_list as) = length (remdups as)"
 proof(induct as)
   case Nil
   then show ?case
@@ -91,17 +91,17 @@ next
     by (simp add: fset_of_list.rep_eq insert_absorb)
 qed
 
-lemma fMax_fold[code]: "fMax (fset_of_list (a#as)) = fold max as a"
+lemma fMax_fold [code]: "fMax (fset_of_list (a#as)) = fold max as a"
   by (metis Max.set_eq_fold fMax.F.rep_eq fset_of_list.rep_eq)
 
-lemma sorted_list_of_fset_sort[code]: "sorted_list_of_fset (fset_of_list as) = sort (remdups as)"
+lemma sorted_list_of_fset_sort [code]: "sorted_list_of_fset (fset_of_list as) = sort (remdups as)"
   by (metis fset_of_list.rep_eq sorted_list_of_fset.rep_eq sorted_list_of_set_sort_remdups)
 
-lemma fremove_code[code]: "fremove a (fset_of_list A) = fset_of_list (filter (\<lambda>x. x \<noteq> a) A)"
+lemma fremove_code [code]: "fremove a (fset_of_list A) = fset_of_list (filter (\<lambda>x. x \<noteq> a) A)"
   apply (simp add: fremove_def minus_fset_def ffilter_def fset_both_sides Abs_fset_inverse fset_of_list.rep_eq)
   by auto
 
-lemma fsubseteq[code]: "(fset_of_list l) |\<subseteq>| A = List.list_all (\<lambda>x. x |\<in>| A) l"
+lemma fsubseteq [code]: "(fset_of_list l) |\<subseteq>| A = List.list_all (\<lambda>x. x |\<in>| A) l"
 proof(induct l)
 case Nil
   then show ?case
@@ -126,11 +126,8 @@ next
     by (simp add: add.commute fold_plus_sum_list_rev fset_of_list.rep_eq fsum.F.rep_eq fSum_def)
 qed
 
-lemma fset_eq: "(x = y) = (x |\<subseteq>| y \<and> size x = size y)"
-  by (metis exists_least_iff le_less size_fsubset)
-
 lemma code_fset_eq [code]: "HOL.equal X (fset_of_list Y) \<longleftrightarrow> size X = length (remdups Y) \<and> (\<forall>x |\<in>| X. List.member Y x)"
-  apply (simp only: HOL.equal_class.equal_eq fset_eq)
+  apply (simp only: HOL.equal_class.equal_eq fset_eq_alt)
   apply (simp only: size)
   using fmember by fastforce
 
